src/paranoid_syntax.v
@@ -20,14 +20,14 @@ Context `{configPrecond : config.Precond}.
 Context `{configReflection : config.Reflection}.
 Context `{configSimpleProducts : config.SimpleProducts}.
 Context `{configProdEta : config.ProdEta}.
-Context `{ConfigUniverses : config.Universes}.
-Context `{ConfigWithProp : config.WithProp}.
-Context `{ConfigId : config.IdentityTypes}.
-Context `{ConfigWithJ : config.WithJ}.
-Context `{ConfigEmpty : config.WithEmpty}.
-Context `{ConfigUnit : config.WithUnit}.
-Context `{ConfigBool : config.WithBool}.
-Context `{ConfigPi : config.WithPi}.
+Context `{configUniverses : config.Universes}.
+Context `{configWithProp : config.WithProp}.
+Context `{configId : config.IdentityTypes}.
+Context `{configWithJ : config.WithJ}.
+Context `{configEmpty : config.WithEmpty}.
+Context `{configUnit : config.WithUnit}.
+Context `{configBool : config.WithBool}.
+Context `{configPi : config.WithPi}.
 
 Inductive context : Type :=
      | ctxempty : context
